list_of_vlsms.v
@@ -1,0 +1,215 @@
+Require Import List.
+Import ListNotations.
+
+From Casper
+Require Import vlsm.
+
+
+Definition composed_state {message} (Ss : list (VLSM message)) : Type :=
+  fold_right prod unit (List.map (@state message) Ss).
+
+Definition composed_label {message} (Ss : list (VLSM message)) : Type :=
+  fold_right sum Empty_set (List.map (@label message) Ss).
+
+Definition composed_proto_message_prop
+  {message}
+  (Ss : list (VLSM message))
+  (m : message) : Prop
+  :=
+  List.Exists (fun s => (@proto_message_prop message s m)) Ss.
+
+Lemma composed_proto_message_decidable
+  {message}
+  (Ss : list (VLSM message))
+  : forall m : message, {composed_proto_message_prop Ss m} + {~composed_proto_message_prop Ss m}.
+Proof.
+  intros.
+  apply Exists_dec. intros s.
+  apply proto_message_decidable.
+Qed.
+
+Definition composed_proto_message
+  {message}
+  (Ss : list (VLSM message))
+  := { m : message | composed_proto_message_prop Ss m }.
+
+Fixpoint composed_initial_state_prop
+  {message}
+  (Ss : list (VLSM message))
+  : composed_state Ss -> Prop.
+destruct Ss as [|Sh St]; unfold composed_state; simpl; intros.
+- exact True.
+- destruct X as [sh st].
+  exact (@initial_state_prop _ Sh sh /\ composed_initial_state_prop _ St st).
+Defined.
+
+Definition composed_initial_state
+  {message}
+  (Ss : list (VLSM message))
+  := { s : composed_state Ss | composed_initial_state_prop Ss s }.
+
+Lemma composed_protocol_state_inhabited
+  {message}
+  (Ss : list (VLSM message))
+  : inhabited (composed_initial_state Ss).
+Proof.
+  induction Ss as [| Sh St IHt].
+  - constructor. exists tt. exact I.
+  - destruct IHt as [[it Hit]].
+    destruct (@protocol_state_inhabited _ Sh) as [[ih Hih]].
+    constructor. exists (ih, it). split; assumption.
+Qed.
+
+Fixpoint composed_initial_message_prop
+  {message}
+  (Ss : list (VLSM message))
+  : composed_proto_message Ss -> Prop.
+destruct Ss as [|Sh St]; unfold composed_state; simpl; intros m.
+- exact False.
+- destruct m as [m Hm].
+  destruct (@proto_message_decidable _ Sh m) as [Hh | _]; destruct (composed_proto_message_decidable St m) as [Ht | _].
+  + exact (initial_message_prop (exist _ m Hh) \/ composed_initial_message_prop _ St (exist _ m Ht)).
+  + exact (initial_message_prop (exist _ m Hh)).
+  + exact (composed_initial_message_prop _ St (exist _ m Ht)).
+  + exact False.
+Defined.
+
+Lemma composed_message_inhabited
+  {message}
+  (Ss : list (VLSM message))
+  (Ssnn : Ss <> [])
+  : inhabited (composed_proto_message Ss)
+  .
+Proof.
+  destruct Ss as [| Sh St]; try contradiction.
+  destruct (@message_inhabited _ Sh) as [[m Hm]].
+  constructor.
+  exists m. apply Exists_cons_hd. assumption.
+Qed.
+
+Lemma composed_label_inhabited
+  {message}
+  (Ss : list (VLSM message))
+  (Ssnn : Ss <> [])
+  : inhabited (composed_label Ss).
+Proof.
+  destruct Ss as [| Sh St]; try contradiction.
+  destruct (@label_inhabited message Sh) as [l].
+  constructor. left. exact l.
+Qed.
+
+Definition lift_proto_messageH
+  {message}
+  (Sh : VLSM message)
+  (St : list (VLSM message))
+  (mh : @proto_message _ Sh)
+  : composed_proto_message (Sh :: St).
+destruct mh as [mh Hmh].
+exists mh.
+apply Exists_cons_hd. assumption.
+Defined.
+
+Definition lift_proto_messageT
+  {message}
+  (Sh : VLSM message)
+  (St : list (VLSM message))
+  (mt : composed_proto_message St)
+  : composed_proto_message (Sh :: St).
+destruct mt as [mt Hmt].
+exists mt.
+apply Exists_cons_tl. assumption.
+Defined.
+
+Fixpoint composed_transition
+  {message}
+  (Ss : list (VLSM message))
+  : composed_label Ss -> composed_state Ss * option (composed_proto_message Ss) -> composed_state Ss * option (composed_proto_message Ss).
+destruct Ss as [| Sh St]; unfold composed_label; unfold composed_state; simpl
+; intros l [s om].
+- inversion l.
+- destruct s as [sh st]. destruct om as [[m Hm]|].
+  + destruct l as [lh | lt].
+    * destruct (@proto_message_decidable _ Sh m) as [Hh | _].
+      { remember (transition lh (sh, Some (exist _ m Hh))) as som'.
+        exact ((fst som', st), option_map (lift_proto_messageH Sh St) (snd som')).
+      }
+      exact ((sh, st), None).
+    * destruct (composed_proto_message_decidable St m) as [Ht | _].
+      { remember (composed_transition _ St lt (st, Some (exist _ m Ht))) as som'.
+        exact ((sh, fst som'), option_map (lift_proto_messageT Sh St) (snd som')).
+      }
+      exact ((sh, st), None).
+  + destruct l as [lh | lt].
+    * remember (transition lh (sh, None)) as som'.
+      exact ((fst som', st), option_map (lift_proto_messageH Sh St) (snd som')).
+    * remember (composed_transition _ St lt (st, None)) as som'.
+      exact ((sh, fst som'), option_map (lift_proto_messageT Sh St) (snd som')).
+Defined.
+
+Fixpoint composed_valid
+  {message}
+  (Ss : list (VLSM message))
+  : composed_label Ss -> composed_state Ss * option (composed_proto_message Ss) -> Prop.
+destruct Ss as [| Sh St]; unfold composed_label; unfold composed_state; simpl
+; intros l [s om].
+- inversion l.
+- destruct s as [sh st]. destruct om as [[m Hm]|].
+  + destruct l as [lh | lt].
+    * destruct (@proto_message_decidable _ Sh m) as [Hh | _].
+      { exact (valid lh (sh, Some (exist _ m Hh))). }
+      exact False.
+    * destruct (composed_proto_message_decidable St m) as [Ht | _].
+      { exact (composed_valid _ St lt (st, Some (exist _ m Ht))). }
+      exact False.
+  + destruct l as [lh | lt].
+    * exact (valid lh (sh, None)).
+    * exact (composed_valid _ St lt (st, None)).
+Defined.
+
+Definition composed_valid_constrained
+  {message}
+  (Ss : list (VLSM message))
+  (constraint : composed_label Ss -> composed_state Ss * option (composed_proto_message Ss) -> Prop)
+  (l : composed_label Ss)
+  (som : composed_state Ss * option (composed_proto_message Ss) )
+  :=
+  composed_valid Ss l som /\ constraint l som.
+
+Definition composed_vlsm
+  {message}
+  (Ss : list (VLSM message))
+  (Ssnn : Ss <> [])
+  : VLSM message
+  :=
+  {| state := composed_state Ss
+  ; label := composed_label Ss
+  ; proto_message_prop := composed_proto_message_prop Ss
+  ; proto_message_decidable := composed_proto_message_decidable Ss
+  ; initial_state_prop := composed_initial_state_prop Ss
+  ; protocol_state_inhabited := composed_protocol_state_inhabited Ss
+  ; initial_message_prop := composed_initial_message_prop Ss
+  ; message_inhabited := composed_message_inhabited Ss Ssnn
+  ; label_inhabited := composed_label_inhabited Ss Ssnn
+  ; transition := composed_transition Ss
+  ; valid := composed_valid Ss
+  |}.
+
+Definition composed_vlsm_constrained
+  {message}
+  (Ss : list (VLSM message))
+  (Ssnn : Ss <> [])
+  (constraint : composed_label Ss -> composed_state Ss * option (composed_proto_message Ss) -> Prop)
+  : VLSM message
+  :=
+  {| state := composed_state Ss
+  ; label := composed_label Ss
+  ; proto_message_prop := composed_proto_message_prop Ss
+  ; proto_message_decidable := composed_proto_message_decidable Ss
+  ; initial_state_prop := composed_initial_state_prop Ss
+  ; protocol_state_inhabited := composed_protocol_state_inhabited Ss
+  ; initial_message_prop := composed_initial_message_prop Ss
+  ; message_inhabited := composed_message_inhabited Ss Ssnn
+  ; label_inhabited := composed_label_inhabited Ss Ssnn
+  ; transition := composed_transition Ss
+  ; valid := composed_valid_constrained Ss constraint
+  |}.
