two_vlsms.v
@@ -1,0 +1,211 @@
+From Casper
+Require Import vlsm.
+
+Definition composed2_proto_message_prop
+  {message}
+  (S1 : VLSM message)
+  (S2 : VLSM message)
+  (m : message) : Prop
+  :=
+  (@proto_message_prop _ S1 m) \/ (@proto_message_prop _ S2 m).
+
+Lemma composed2_proto_message_decidable
+  {message}
+  (S1 : VLSM message)
+  (S2 : VLSM message)
+  : forall m : message, {composed2_proto_message_prop S1 S2 m} + {~ composed2_proto_message_prop S1 S2 m}.
+Proof.
+  intros.
+  destruct (@proto_message_decidable _ S1 m) as [Hm1 | Hm1'].
+  - left. left. assumption.
+  - destruct (@proto_message_decidable _ S2 m) as [Hm2 | Hm2'].
+    + left. right. apply Hm2.
+    + right. intros H. destruct H as [H | H]; contradiction.
+Qed.
+
+Definition composed2_proto_message
+  {message}
+  (S1 : VLSM message)
+  (S2 : VLSM message)
+  :=
+  { m : message | composed2_proto_message_prop S1 S2 m }.
+
+Definition composed2_initial_state_prop
+  {message}
+  (S1 : VLSM message)
+  (S2 : VLSM message)
+  (s : (@state message S1) * (@state message S2)) : Prop
+  :=
+  match s with
+  | (s1, s2) => initial_state_prop s1 /\ initial_state_prop s2
+  end.
+
+Definition composed2_initial_state
+  {message}
+  (S1 : VLSM message)
+  (S2 : VLSM message)
+  :=
+  { s : (@state message S1) * (@state message S2) | composed2_initial_state_prop S1 S2 s }.
+
+Lemma composed2_protocol_state_inhabited
+  {message}
+  (S1 : VLSM message)
+  (S2 : VLSM message)
+  : inhabited (composed2_initial_state S1 S2).
+Proof.
+  destruct (@protocol_state_inhabited message S1) as [s1].
+  destruct (@protocol_state_inhabited message S2) as [s2].
+  destruct s1 as [i1 Hi1]. destruct s2 as [i2 Hi2].
+  constructor. exists (i1, i2). split; assumption.
+Qed.
+
+Definition composed2_initial_message_prop
+  {message}
+  (S1 : VLSM message)
+  (S2 : VLSM message)
+  (m : composed2_proto_message S1 S2) : Prop.
+destruct m as [m Hm].
+destruct (@proto_message_decidable _ S1 m) as [H1 | _]; destruct (@proto_message_decidable _ S2 m) as [H2 | _].
+- exact (initial_message_prop (exist _ m H1) \/ initial_message_prop (exist _ m H2)).
+- exact (initial_message_prop (exist _ m H1)).
+- exact (initial_message_prop (exist _ m H2)).
+- exact False.
+Defined.
+
+Lemma composed2_message_inhabited
+  {message}
+  (S1 : VLSM message)
+  (S2 : VLSM message)
+  : inhabited (composed2_proto_message S1 S2)
+  .
+Proof.
+  destruct (@message_inhabited message S1) as [[m Hm]].
+  constructor.  exists m. left. assumption.
+Qed.
+
+Lemma composed2_label_inhabited
+  {message}
+  (S1 : VLSM message)
+  (S2 : VLSM message)
+  : inhabited ((@label message S1) + (@label message S2)).
+Proof.
+  destruct (@label_inhabited message S1) as [l].
+  constructor.  left.  exact l.
+Qed.
+
+
+Definition lift_proto_message1
+  {message}
+  (S1 : VLSM message)
+  (S2 : VLSM message)
+  (m1 : @proto_message _ S1)
+  : composed2_proto_message S1 S2.
+destruct m1 as [m1 Hm1].
+exists m1.
+unfold composed2_proto_message_prop. left. assumption.
+Defined.
+
+
+Definition lift_proto_message2
+  {message}
+  (S1 : VLSM message)
+  (S2 : VLSM message)
+  (m2 : @proto_message _ S2)
+  : composed2_proto_message S1 S2.
+destruct m2 as [m2 Hm2].
+exists m2.
+unfold composed2_proto_message_prop. right. assumption.
+Defined.
+
+Definition composed2_transition
+  {message}
+  (S1 : VLSM message)
+  (S2 : VLSM message)
+  (l : (@label message S1) + (@label message S2))
+  (som : ((@state message S1) * (@state message S2)) * option (composed2_proto_message S1 S2))
+  : (((@state message S1) * (@state message S2)) * option (composed2_proto_message S1 S2))%type.
+destruct som as [[s1 s2] [[m Hm]|]].
+- destruct l as [l1 | l2].
+  + destruct (@proto_message_decidable _ S1 m) as [H1 | _].
+    * remember (transition l1 (s1, Some (exist _ m H1))) as som'.
+      exact ((fst som', s2), option_map (lift_proto_message1 S1 S2) (snd som')).
+    * exact ((s1, s2), None).
+  + destruct (@proto_message_decidable _ S2 m) as [H2 | _].
+    * remember (transition l2 (s2, Some (exist _ m H2))) as som'.
+      exact ((s1, fst som'), option_map (lift_proto_message2 S1 S2) (snd som')).
+    * exact ((s1, s2), None).
+- destruct l as [l1 | l2].
+  + remember (transition l1 (s1, None)) as som'.
+    exact ((fst som', s2), option_map (lift_proto_message1 S1 S2) (snd som')).
+  + remember (transition l2 (s2, None)) as som'.
+      exact ((s1, fst som'), option_map (lift_proto_message2 S1 S2) (snd som')).
+Defined.
+
+Definition composed2_valid
+  {message}
+  (S1 : VLSM message)
+  (S2 : VLSM message)
+  (l : (@label message S1) + (@label message S2))
+  (som : ((@state message S1) * (@state message S2)) * option (composed2_proto_message S1 S2))
+  : Prop.
+destruct som as [[s1 s2] [[m Hm]|]].
+- destruct l as [l1 | l2].
+  + destruct (@proto_message_decidable _ S1 m) as [H1 | _].
+    * exact (valid l1 (s1, Some (exist _ m H1))).
+    * exact False.
+  + destruct (@proto_message_decidable _ S2 m) as [H2 | _].
+    * exact (valid l2 (s2, Some (exist _ m H2))).
+    * exact False.
+- destruct l as [l1 | l2].
+  + exact (valid l1 (s1, None)).
+  + exact (valid l2 (s2, None)).
+Defined.
+
+Definition composed2_valid_constrained
+  {message}
+  (S1 : VLSM message)
+  (S2 : VLSM message)
+  (constraint : (@label message S1) + (@label message S2) -> ((@state message S1) * (@state message S2)) * option (composed2_proto_message S1 S2) -> Prop)
+  (l : (@label message S1) + (@label message S2))
+  (som : ((@state message S1) * (@state message S2)) * option (composed2_proto_message S1 S2))
+  :=
+  composed2_valid S1 S2 l som /\ constraint l som.
+
+Definition compose2_vlsm
+  {message}
+  (S1 : VLSM message)
+  (S2 : VLSM message)
+  : VLSM message
+  :=
+  {| state := (@state message S1) * (@state message S2)
+  ; label := (@label message S1) + (@label message S2)
+  ; proto_message_prop := composed2_proto_message_prop S1 S2
+  ; proto_message_decidable := composed2_proto_message_decidable S1 S2
+  ; initial_state_prop := composed2_initial_state_prop S1 S2
+  ; protocol_state_inhabited := composed2_protocol_state_inhabited S1 S2
+  ; initial_message_prop := composed2_initial_message_prop S1 S2
+  ; message_inhabited := composed2_message_inhabited S1 S2
+  ; label_inhabited := composed2_label_inhabited S1 S2
+  ; transition := composed2_transition S1 S2
+  ; valid := composed2_valid S1 S2
+  |}.
+
+Definition compose2_vlsm_constrained
+  {message}
+  (S1 : VLSM message)
+  (S2 : VLSM message)
+  (constraint : (@label message S1) + (@label message S2) -> (@state message S1 * @state message S2) * option (composed2_proto_message S1 S2) -> Prop)
+  : VLSM message
+  :=
+  {| state := (@state message S1) * (@state message S2)
+  ; label := (@label message S1) + (@label message S2)
+  ; proto_message_prop := composed2_proto_message_prop S1 S2
+  ; proto_message_decidable := composed2_proto_message_decidable S1 S2
+  ; initial_state_prop := composed2_initial_state_prop S1 S2
+  ; protocol_state_inhabited := composed2_protocol_state_inhabited S1 S2
+  ; initial_message_prop := composed2_initial_message_prop S1 S2
+  ; message_inhabited := composed2_message_inhabited S1 S2
+  ; label_inhabited := composed2_label_inhabited S1 S2
+  ; transition := composed2_transition S1 S2
+  ; valid := composed2_valid_constrained S1 S2 constraint
+  |}.
