Makefile
@@ -3,7 +3,7 @@ COQDEP = coqdep
 
 COQ_FLAG = -Q "." Casper
 
-SOURCE := preamble.v ListExtras.v ListSetExtras.v RealsExtras.v sorted_lists.v protocol.v common.v definitions.v fullnode.v lightnode.v binary.v ctl.v vlsm.v
+SOURCE := preamble.v ListExtras.v ListSetExtras.v RealsExtras.v sorted_lists.v protocol.v common.v definitions.v fullnode.v lightnode.v binary.v ctl.v vlsm.v two_vlsms.v list_of_vlsms.v indexed_vlsm.v
 VO_FILE := $(shell find "." -type f -name '*.vo')
 GLOB_FILE := $(shell find "." -type f -name '*.glob')
 AUX_FILE := $(shell find "." -type f -name '*.vo.aux')
@@ -13,7 +13,7 @@ $(SOURCE:%.v=%.vo): %.vo: %.v
 			@$(COQC) $(COQ_FLAG) $*.v
 
 dep:
-	@$(COQDEP) $(SOURCE) > .depend
+	@$(COQDEP) $(COQ_FLAG) $(SOURCE) > .depend
 
 all: $(SOURCE:%.v=%.vo)
 	
